add some simple stuff to sketchScript

sketchScript.sml
@@ -1,4 +1,5 @@
 open HolKernel boolLib bossLib lcsymtacs
+open pred_setTheory
 open holSemanticsTheory
 
 val _ = temp_tight_equality()
@@ -16,6 +17,21 @@ val finv_def = Define`
 val range_def = Define`
   range0 ^mem (f : α -> 'U) = @x. BIJ f UNIV {a | mem a x}`
 val _ = Parse.overload_on("range",``range0 ^mem``)
+
+val in_bool_def = Define`
+  in_bool0 ^mem = Boolean`
+val _ = Parse.overload_on("in_bool",``in_bool0 ^mem``)
+
+(*
+val in_bool_is_bij = store_thm("in_bool_is_bij",
+  ``is_set_theory ^mem ==> BIJ in_bool UNIV (ext (range in_bool))``,
+  rw[in_bool_def,ext_def,range_def,BIJ_IFF_INV] >- (
+
+    rw[in_bool_def,boolean_in_boolset] ) >>
+  qexists_tac`λx. x = True` >>
+  rw[in_bool_def,boolean_eq_true] >>
+  rfs[mem_boolset,boolean_eq_true,true_neq_false,boolean_def])
+*)
 
 val in_fun_def = Define`
   in_fun0 ^mem ina inb f =
@@ -46,5 +62,46 @@ val example =
     ⇒
     in_fun in_α (in_fun in_β in_ind) P =
        termsem ^tmsig (tyass,tmass) (tyval,tmval) ^P_deep``
+
+val example_sequent =
+  ( [ ``is_set_theory ^mem``
+    , ``is_interpretation (^tysig,^tmsig) (tyass,tmass)``
+    , ``is_std_interpretation (tyass,tmass)``
+    , ``is_valuation ^tysig tmass (tyval,tmval)``
+    , ``BIJ (in_α : α -> 'U) UNIV (ext (tyval "'a"))``
+    , ``BIJ (in_β : β -> 'U) UNIV (ext (tyval "'b"))``
+    , ``BIJ (in_ind : ind -> 'U) UNIV (ext (tyass "ind" []))``
+    , ``BIJ (in_list_α : α list -> 'U) UNIV (ext (tyass "list" [tyval "'a"]))``
+    , ``tmass "c" [range (in_fun in_α in_β)] = in_fun in_α in_β c``
+    , ``tmval ("x",Fun Ind Ind) = in_fun in_ind in_ind x``
+    ]
+  , ``in_fun in_α (in_fun in_β in_ind) P =
+        termsem ^tmsig (tyass,tmass) (tyval,tmval) ^P_deep`` )
+
+
+fun underscores [] = ""
+  | underscores (x::xs) = "_" ^ x ^ underscores xs
+
+fun type_name (ty : hol_type) =
+  if is_type ty then case dest_thy_type ty of
+    { Args = args, Thy = thy, Tyop = tyop } =>
+      tyop ^ underscores (map type_name args)
+  else
+    dest_vartype ty
+
+fun mk_in_var (ty : hol_type) =
+  mk_var ("in_" ^ type_name ty, ``:^(ty) -> 'U``)
+
+fun mk_in (ty : hol_type) =
+  if is_type ty then case dest_thy_type ty of
+      { Args = [], Thy = thy, Tyop = "bool" } =>
+        ``in_bool``
+    | { Args = [ty1,ty2], Thy = thy, Tyop = "fun" } =>
+        ``in_fun ^(mk_in ty1) ^(mk_in ty2)``
+    | { Args = args, Thy = thy, Tyop = tyop } =>
+        mk_in_var ty
+  else
+    mk_in_var ty
+ 
 
 val _ = export_theory()
